coq/cNRAEnv/Lang/cNRAEnv.v
@@ -14,6 +14,28 @@
  * limitations under the License.
  *)
 
+(** cNRAEnv is the Core Nested Relational Algebra with
+Environments. *)
+
+(** cNRAEnv is a small pure language without functions based on
+combinators (i.e., with no variables). Expressions in cNRAEnv take two
+values as input, a current value and a value that can encode an
+environment. *)
+
+(** Summary:
+- Language: cNRAEnv (Core Nested Relational Algebra with Environments)
+- Based on: "Handling Environments in a Nested Relational Algebra with
+  Combinators and an Implementation in a Verified Query Compiler", by
+  Joshua Auerbach, Martin Hirzel, Louis Mandel, Avraham Shinnar and
+  Jérôme Siméon (ACM SIGMOD'2017 conference).
+- translating to cNRAEnv: CAMP, NRA, NRAEnv
+- translating from cNRAEnv: cNNRC, NRAEnv *)
+
+(** Compared to the version from Hirzel et al:
+- We add two operators for matching against either values ([Either]
+  and [EitherConcat]).
+*)
+
 Section cNRAEnv.
   Require Import String.
   Require Import List.
@@ -22,431 +44,1070 @@ Section cNRAEnv.
   Require Import Utils.
   Require Import CommonRuntime.
 
-  (** Nested Relational Algebra *)
-
-  (** By convention, "static" parameters come first, followed by
-     dependent operators. This allows for instanciation on those
-     parameters *)
-
   Context {fruntime:foreign_runtime}.
 
-  Inductive nraenv_core : Set :=
-  | cNRAEnvID : nraenv_core
-  | cNRAEnvConst : data -> nraenv_core
-  | cNRAEnvBinop : binary_op -> nraenv_core -> nraenv_core -> nraenv_core
-  | cNRAEnvUnop : unary_op -> nraenv_core -> nraenv_core
-  | cNRAEnvMap : nraenv_core -> nraenv_core -> nraenv_core
-  | cNRAEnvMapProduct : nraenv_core -> nraenv_core -> nraenv_core
-  | cNRAEnvProduct : nraenv_core -> nraenv_core -> nraenv_core
-  | cNRAEnvSelect : nraenv_core -> nraenv_core -> nraenv_core
-  | cNRAEnvDefault : nraenv_core -> nraenv_core -> nraenv_core
-  | cNRAEnvEither :  nraenv_core -> nraenv_core -> nraenv_core
-  | cNRAEnvEitherConcat :  nraenv_core -> nraenv_core -> nraenv_core
-  | cNRAEnvApp : nraenv_core -> nraenv_core -> nraenv_core
-  | cNRAEnvGetConstant : string -> nraenv_core
-  | cNRAEnvEnv : nraenv_core
-  | cNRAEnvAppEnv : nraenv_core -> nraenv_core -> nraenv_core
-  | cNRAEnvMapEnv : nraenv_core -> nraenv_core
-  .
+  (** * Abstract Syntax *)
+
+  Section Syntax.
+  
+  (** By convention, "static" parameters come first, followed by
+     so-called dependent operators. This allows for easy instanciation
+     on those parameters *)
+
+    Inductive nraenv_core : Set :=
+    | cNRAEnvGetConstant : string -> nraenv_core
+    | cNRAEnvID : nraenv_core
+    | cNRAEnvConst : data -> nraenv_core
+    | cNRAEnvBinop : binary_op -> nraenv_core -> nraenv_core -> nraenv_core
+    | cNRAEnvUnop : unary_op -> nraenv_core -> nraenv_core
+    | cNRAEnvMap : nraenv_core -> nraenv_core -> nraenv_core
+    | cNRAEnvMapProduct : nraenv_core -> nraenv_core -> nraenv_core
+    | cNRAEnvProduct : nraenv_core -> nraenv_core -> nraenv_core
+    | cNRAEnvSelect : nraenv_core -> nraenv_core -> nraenv_core
+    | cNRAEnvDefault : nraenv_core -> nraenv_core -> nraenv_core
+    | cNRAEnvEither :  nraenv_core -> nraenv_core -> nraenv_core
+    | cNRAEnvEitherConcat :  nraenv_core -> nraenv_core -> nraenv_core
+    | cNRAEnvApp : nraenv_core -> nraenv_core -> nraenv_core
+    | cNRAEnvEnv : nraenv_core
+    | cNRAEnvAppEnv : nraenv_core -> nraenv_core -> nraenv_core
+    | cNRAEnvMapEnv : nraenv_core -> nraenv_core
+    .
+
+    Global Instance nraenv_core_eqdec : EqDec nraenv_core eq.
+    Proof.
+      change (forall x y : nraenv_core,  {x = y} + {x <> y}).
+      decide equality;
+        try solve [apply binary_op_eqdec | apply unary_op_eqdec | apply data_eqdec | apply string_eqdec].
+    Defined.
+
+  End Syntax.
 
   Tactic Notation "nraenv_core_cases" tactic(first) ident(c) :=
-  first;
-  [ Case_aux c "cNRAEnvID"%string
-  | Case_aux c "cNRAEnvConst"%string
-  | Case_aux c "cNRAEnvBinop"%string
-  | Case_aux c "cNRAEnvUnop"%string
-  | Case_aux c "cNRAEnvMap"%string
-  | Case_aux c "cNRAEnvMapProduct"%string
-  | Case_aux c "cNRAEnvProduct"%string
-  | Case_aux c "cNRAEnvSelect"%string
-  | Case_aux c "cNRAEnvDefault"%string
-  | Case_aux c "cNRAEnvEither"%string
-  | Case_aux c "cNRAEnvEitherConcat"%string
-  | Case_aux c "cNRAEnvApp"%string
-  | Case_aux c "cNRAEnvGetConstant"%string
-  | Case_aux c "cNRAEnvEnv"%string
-  | Case_aux c "cNRAEnvAppEnv"%string
-  | Case_aux c "cNRAEnvMapEnv"%string].
+    first;
+    [ Case_aux c "cNRAEnvGetConstant"%string
+    | Case_aux c "cNRAEnvID"%string
+    | Case_aux c "cNRAEnvConst"%string
+    | Case_aux c "cNRAEnvBinop"%string
+    | Case_aux c "cNRAEnvUnop"%string
+    | Case_aux c "cNRAEnvMap"%string
+    | Case_aux c "cNRAEnvMapProduct"%string
+    | Case_aux c "cNRAEnvProduct"%string
+    | Case_aux c "cNRAEnvSelect"%string
+    | Case_aux c "cNRAEnvDefault"%string
+    | Case_aux c "cNRAEnvEither"%string
+    | Case_aux c "cNRAEnvEitherConcat"%string
+    | Case_aux c "cNRAEnvApp"%string
+    | Case_aux c "cNRAEnvEnv"%string
+    | Case_aux c "cNRAEnvAppEnv"%string
+    | Case_aux c "cNRAEnvMapEnv"%string].
   
-  Global Instance nraenv_core_eqdec : EqDec nraenv_core eq.
-  Proof.
-    change (forall x y : nraenv_core,  {x = y} + {x <> y}).
-    decide equality;
-      try solve [apply binary_op_eqdec | apply unary_op_eqdec | apply data_eqdec | apply string_eqdec].
-  Defined.
+  (** * Semantics *)
+  
+  Section Semantics.
+    (** Part of the context is fixed for the rest of the development:
+- [h] is the brand relation
+- [constant_env] is the global environment *)
 
-  (** NRA+Env Semantics *)
+    Context (h:list(string*string)).
+    Context (constant_env:list (string*data)).
 
-  Context (h:list(string*string)).
-  Context (constant_env:list (string*data)).
-  Fixpoint nraenv_core_eval (op:nraenv_core) (env: data) (x:data) : option data :=
-    match op with
-      | cNRAEnvID => Some x
-      | cNRAEnvConst rd => Some (normalize_data h rd)
-      | cNRAEnvBinop bop op1 op2 =>
-        olift2 (fun d1 d2 => binary_op_eval h bop d1 d2) (nraenv_core_eval op1 env x) (nraenv_core_eval op2 env x)
-      | cNRAEnvUnop uop op1 =>
-        olift (fun d1 => unary_op_eval h uop d1) (nraenv_core_eval op1 env x)
-      | cNRAEnvMap op1 op2 =>
-        let aux_map d :=
-            lift_oncoll (fun c1 => lift dcoll (lift_map (nraenv_core_eval op1 env) c1)) d
-        in olift aux_map (nraenv_core_eval op2 env x)
-      | cNRAEnvMapProduct op1 op2 =>
-        let aux_mapconcat d :=
-            lift_oncoll (fun c1 => lift dcoll (omap_product (nraenv_core_eval op1 env) c1)) d
-        in olift aux_mapconcat (nraenv_core_eval op2 env x)
-      | cNRAEnvProduct op1 op2 =>
+    (** ** Denotational Semantics *)
+
+    (** The semantics is defined using the main judgment [Γc ; γ ; d ⊢
+    〚e〛⇓ d'] ([nraenv_core_sem]) where [Γc] is the global
+    environment, [γ] is the reified input environment, [d] is the
+    input value, [e] the cNRAEnv expression and [d'] the resulting
+    value. *)
+    
+    (** The auxiliary judgment [Γc ; γ ; {c₁} ⊢〚e〛χ ⇓ {c₂}]
+    ([nraenv_core_sem_map]) is used in the definition of the map [χ]
+    operator. *)
+    
+    (** The auxiliary judgment [Γc ; γ ; {c₁} ⊢〚e〛⋈ᵈ ⇓ {c₂}]
+    ([nra_map_product_select]) is used in the definition of the
+    dependant product [⋈ᵈ] operator. *)
+    
+    (** The auxiliary judgment [Γc ; γ ; {c₁} ⊢〚e〛σ ⇓ {c₂}]
+    ([nraenv_core_sem_select]) is used in the definition of the
+    selection [σ] operator. *)
+    
+    (** The auxiliary judgment [Γc ; {c₁} ; d ⊢〚e〛χᵉ ⇓ {c₂}]
+    ([nraenv_core_sem_map_env]) is used in the definition of the map
+    over environment [χᵉ] operator. *)
+    
+    Section Denotation.
+      Inductive nraenv_core_sem: nraenv_core -> data -> data -> data -> Prop :=
+      | sem_cNRAEnvGetConstant : forall v env d d1,
+          edot constant_env v = Some d1 ->                   (**r   [Γc(v) = d₁] *)
+          nraenv_core_sem (cNRAEnvGetConstant v) env d d1    (**r ⇒ [Γc ; γ ; d ⊢〚$$v〛⇓ d₁] *)
+      | sem_cNRAEnvID : forall env d,
+          nraenv_core_sem cNRAEnvID env d d                  (**r   [Γc ; γ ; d ⊢ ID ⇓ d] *)
+      | sem_cNRAEnvConst : forall env d d1 d2,
+          normalize_data h d1 = d2 ->                        (**r   [norm(d₁) = d₂] *)
+          nraenv_core_sem (cNRAEnvConst d1) env d d2         (**r ⇒ [Γc ; γ ; d ⊢〚d₁〛⇓ d₂] *)
+      | sem_cNRAEnvBinop : forall bop e1 e2 env d d1 d2 d3,
+          nraenv_core_sem e1 env d d1 ->                     (**r   [Γc ; γ ; d ⊢〚e₁〛⇓ d₁] *)
+          nraenv_core_sem e2 env d d2 ->                     (**r ∧ [Γc ; γ ; d ⊢〚e₂〛⇓ d₂] *)
+          binary_op_eval h bop d1 d2 = Some d3 ->            (**r ∧ [d₁ ⊠ d₂ = d₃] *)
+          nraenv_core_sem (cNRAEnvBinop bop e1 e2) env d d3  (**r ⇒ [Γc ; γ ; d ⊢〚e₁ ⊠ e₂〛⇓ d₃] *)
+      | sem_cNRAEnvUnop : forall uop e env d d1 d2,
+          nraenv_core_sem e env d d1 ->                      (**r   [Γc ; γ ; d ⊢〚e〛⇓ d₁] *)
+          unary_op_eval h uop d1 = Some d2 ->                (**r ∧ [⊞ d₁ = d₂] *)
+          nraenv_core_sem (cNRAEnvUnop uop e) env d d2       (**r ⇒ [Γc ; γ ; d ⊢〚⊞ e〛⇓ d₂] *)
+      | sem_cNRAEnvMap : forall e1 e2 env d c1 c2,
+          nraenv_core_sem e1 env d (dcoll c1) ->             (**r   [Γc ; γ ; d ⊢〚e₁〛⇓ {c₁}] *)
+          nraenv_core_sem_map e2 env c1 c2 ->                (**r ∧ [Γc ; γ ; {c₁} ⊢〚e₂〛χ ⇓ {c₂}] *)
+          nraenv_core_sem (cNRAEnvMap e2 e1) env d (dcoll c2)(**r ⇒ [Γc ; γ ; d ⊢〚χ⟨e₂⟩(e₁)〛⇓ {c₂}] *)
+      | sem_cNRAEnvMapProduct : forall e1 e2 env d c1 c2,
+          nraenv_core_sem e1 env d (dcoll c1) ->             (**r   [Γc ; γ ; d ⊢〚e₁〛⇓ {c₁}] *)
+          nraenv_core_sem_map_product e2 env c1 c2 ->        (**r ∧ [Γc ; γ ; {c₁} ⊢〚e₂〛⋈ᵈ ⇓ {c₂}] *)
+          nraenv_core_sem                                    (**r ⇒ [Γc ; γ ; d ⊢〚⋈ᵈ⟨e₂⟩(e₁)〛⇓ {c₂}] *)
+            (cNRAEnvMapProduct e2 e1) env d (dcoll c2)
+      | sem_cNRAEnvProduct_empty : forall e1 e2 env d,       (**r Does not evaluate [e₂] if [e₁] is empty. This facilitates translation to cNNRC *)
+          nraenv_core_sem e1 env d (dcoll nil) ->            (**r   [Γc ; γ ; d ⊢〚e₁〛⇓ {}] *)
+          nraenv_core_sem                                    (**r ⇒ [Γc ; γ ; d ⊢〚e₁ × e₂〛⇓ {}] *)
+            (cNRAEnvProduct e1 e2) env d (dcoll nil)
+      | sem_cNRAEnvProduct_nonEmpty : forall e1 e2 env d c1 c2 c3,
+          nraenv_core_sem e1 env d (dcoll c1) ->             (**r   [Γc ; γ ; d ⊢〚e₁〛⇓ {c₁}] *)
+          c1 <> nil ->                                       (**r ∧ [{c₁} ≠ {}] *)
+          nraenv_core_sem e2 env d (dcoll c2) ->             (**r ∧ [Γc ; γ ; d ⊢〚e₂〛⇓ {c₂}] *)
+          product_sem c1 c2 c3 ->                            (**r ∧ [{c₁} × {c₂} ⇓ {c₃}] *)
+          nraenv_core_sem                                    (**r ⇒ [Γc ; γ ; d ⊢〚e₁ × e₂〛⇓ {c₃}] *)
+            (cNRAEnvProduct e1 e2) env d (dcoll c3)
+      | sem_cNRAEnvSelect : forall e1 e2 env d c1 c2,
+          nraenv_core_sem e1 env d (dcoll c1) ->             (**r   [Γc ; γ ; d ⊢〚e₁〛⇓ {c₁}] *)
+          nraenv_core_sem_select e2 env c1 c2 ->             (**r ∧ [Γc ; γ ; {c₁} ⊢〚e₂〛σ ⇓ {c₂}] *)
+          nraenv_core_sem                                    (**r ⇒ [Γc ; γ ; d ⊢〚σ⟨e₂⟩(e₁)〛⇓ {c₂}] *)
+            (cNRAEnvSelect e2 e1) env d (dcoll c2)
+      | sem_cNRAEnvDefault_empty : forall e1 e2 env d d2,
+          nraenv_core_sem e1 env d  (dcoll nil) ->           (**r   [Γc ; γ ; d ⊢〚e₁〛⇓ {}] *)
+          nraenv_core_sem e2 env d d2 ->                     (**r ∧ [Γc ; γ ; d ⊢〚e₂〛⇓ d₂] *)
+          nraenv_core_sem (cNRAEnvDefault e1 e2) env d d2    (**r ⇒ [Γc ; γ ; d ⊢〚e₁ ∥ e₂〛⇓ d₂] *)
+      | sem_cNRAEnvDefault_not_empty : forall e1 e2 env d d1,
+          nraenv_core_sem e1 env d d1 ->                     (**r   [Γc ; γ ; d ⊢〚e₁〛⇓ d₁] *)
+          d1 <> dcoll nil ->                                 (**r ∧ [d₁ ≠ {}] *)
+          nraenv_core_sem (cNRAEnvDefault e1 e2) env d d1    (**r ⇒ [Γc ; γ ; d ⊢〚e₁ ∥ e₂〛⇓ d₁] *)
+      | sem_cNRAEnvEither_left : forall e1 e2 env d d1,
+          nraenv_core_sem e1 env d d1 ->                     (**r   [Γc ; γ ; d ⊢〚e₁〛⇓ d₁] *)
+          nraenv_core_sem                                    (**r ⇒ [Γc ; γ ; (dleft d) ⊢〚either e₁ e₂〛⇓ d₁] *)
+            (cNRAEnvEither e1 e2) env (dleft d) d1
+      | sem_cNRAEnvEither_right : forall e1 e2 env d d2,
+          nraenv_core_sem e2 env d d2 ->                     (**r   [Γc ; γ ; d ⊢〚e₂〛⇓ d₂] *)
+          nraenv_core_sem                                    (**r ⇒ [Γc ; γ ; (dright d) ⊢〚either e₁ e₂〛⇓ d₂] *)
+            (cNRAEnvEither e1 e2) env (dright d) d2
+      | sem_cNRAEnvEitherConcat_left : forall e1 e2 env d r1 r2,
+          nraenv_core_sem e1 env d (dleft (drec r1)) ->      (**r   [Γc ; γ ; d ⊢〚e₁〛⇓ (dleft [r₁])] *)
+          nraenv_core_sem e2 env d (drec r2) ->              (**r ∧ [Γc ; γ ; d ⊢〚e₂〛⇓ [r₂]] *)
+          nraenv_core_sem                                    (**r ⇒ [Γc ; γ ; d ⊢〚either⊕ e₁ e₂〛⇓ (dleft [r₁]⊕[r₂]]) *)
+            (cNRAEnvEitherConcat e1 e2) env d
+            (dleft (drec (rec_concat_sort r1 r2)))
+      | sem_cNRAEnvEitherConcat_right : forall e1 e2 env d r1 r2,
+          nraenv_core_sem e1 env d (dright (drec r1)) ->     (**r   [Γc ; γ ; d ⊢〚e₁〛⇓ (dright [r₁])] *)
+          nraenv_core_sem e2 env d (drec r2) ->              (**r ∧ [Γc ; γ ; d ⊢〚e₂〛⇓ [r₂]] *)
+          nraenv_core_sem                                    (**r ⇒ [Γc ; γ ; d ⊢〚either⊕ e₁ e₂〛⇓ (dright [r₁]⊕[r₂]]) *)
+            (cNRAEnvEitherConcat e1 e2) env d
+            (dright (drec (rec_concat_sort r1 r2)))
+      | sem_cNRAEnvApp : forall e1 e2 env d d1 d2,
+          nraenv_core_sem e1 env d d1 ->                     (**r   [Γc ; γ ; d ⊢〚e₁〛⇓ d₁] *)
+          nraenv_core_sem e2 env d1 d2 ->                    (**r   [Γc ; γ ; d₁ ⊢〚e₂〛⇓ d₂] *)
+          nraenv_core_sem (cNRAEnvApp e2 e1) env d d2        (**r ⇒ [Γc ; γ ; d ⊢〚e₂ ∘ e₁〛⇓ d₂] *)
+      | sem_cNRAEnvEnv : forall env d,
+          nraenv_core_sem cNRAEnvEnv env d env               (**r   [Γc ; γ ; d ⊢ ENV ⇓ γ] *)
+      | sem_cNRAEnvAppEnv : forall e1 e2 env d env1 d2,
+          nraenv_core_sem e1 env d env1 ->                   (**r   [Γc ; γ ; d ⊢〚e₁〛⇓ γ₁] *)
+          nraenv_core_sem e2 env1 d d2 ->                    (**r   [Γc ; γ₁ ; d ⊢〚e₂〛⇓ d₂] *)
+          nraenv_core_sem (cNRAEnvAppEnv e2 e1) env d d2     (**r ⇒ [Γc ; γ ; d ⊢〚e₂ ∘ᵉ e₁〛⇓ d₂] *)
+      | sem_cNRAEnvMapEnv : forall e c1 d c2,
+          nraenv_core_sem_map_env e c1 d c2 ->               (**r ∧ [Γc ; {c₁} ; d ⊢〚e〛χᵉ ⇓ {c₂}] *)
+          nraenv_core_sem                                    (**r ⇒ [Γc ; {c₁} ; d ⊢〚χᵉ⟨e⟩〛⇓ {c₂}] *)
+            (cNRAEnvMapEnv e) (dcoll c1) d (dcoll c2)
+      with nraenv_core_sem_map: nraenv_core -> data -> list data -> list data -> Prop :=
+      | sem_cNRAEnvMap_empty : forall e env,
+          nraenv_core_sem_map e env nil nil                     (**r   [Γc ; γ ; {} ⊢〚e〛χ ⇓ {}] *)
+      | sem_cNRAEnvMap_cons : forall e env d1 c1 d2 c2,
+          nraenv_core_sem e env d1 d2 ->                        (**r   [Γc ; γ ; d₁ ⊢〚e〛⇓ d₂]  *)
+          nraenv_core_sem_map e env c1 c2 ->                    (**r ∧ [Γc ; γ ; {c₁} ⊢〚e〛χ ⇓ {c₂}] *)
+          nraenv_core_sem_map e env (d1::c1) (d2::c2)           (**r ⇒ [Γc ; γ ; {d₁::c₁} ⊢〚e〛χ ⇓ {d₂::c₂}] *)
+      with nraenv_core_sem_map_product: nraenv_core -> data -> list data -> list data -> Prop :=
+      | sem_cNRAEnvMapProduct_empty : forall e env,
+          nraenv_core_sem_map_product e env nil nil             (**r   [Γc ; γ ; {} ⊢〚e〛⋈ᵈ ⇓ {}] *)
+      | sem_cNRAEnvMapProduct_cons : forall e env d1 c1 c2 c3 c4,
+          nraenv_core_sem e env d1 (dcoll c3) ->                (**r   [Γc ; γ ; d₁ ⊢〚e〛⋈ᵈ ⇓ {c₃}]  *)
+          map_concat_sem d1 c3 c4 ->                            (**r ∧ [d₁ χ⊕ c₃ ⇓ c₄] *)
+          nraenv_core_sem_map_product e env c1 c2 ->            (**r ∧ [Γc ; γ ; {c₁} ⊢〚e〛⋈ᵈ ⇓ {c₂}] *)
+          nraenv_core_sem_map_product e env (d1::c1) (c4 ++ c2) (**r ⇒ [Γc ; γ ; {d₁::c₁} ⊢〚e〛⋈ᵈ ⇓ {c₄}∪{c₂}] *)
+      with nraenv_core_sem_select: nraenv_core -> data -> list data -> list data -> Prop :=
+      | sem_cNRAEnvSelect_empty : forall e env,
+          nraenv_core_sem_select e env nil nil                  (**r   [Γc ; γ ; {} ⊢〚e〛σ ⇓ {}] *)
+      | sem_cNRAEnvSelect_true : forall e env d1 c1 c2,
+          nraenv_core_sem e env d1 (dbool true) ->              (**r   [Γc ; γ ; d₁ ⊢〚e〛σ ⇓ true]  *)
+          nraenv_core_sem_select e env c1 c2 ->                 (**r ∧ [Γc ; γ ; {c₁} ⊢〚e〛σ ⇓ {c₂}] *)
+          nraenv_core_sem_select e env (d1::c1) (d1::c2)        (**r ⇒ [Γc ; γ ; {d₁::c₁} ⊢〚e〛σ ⇓ {d₁::c₂}] *)
+      | sem_cNRAEnvSelect_false : forall e env d1 c1 c2,
+          nraenv_core_sem e env d1 (dbool false) ->             (**r   [Γc ; γ ; d₁ ⊢〚e〛σ ⇓ false]  *)
+          nraenv_core_sem_select e env c1 c2 ->                 (**r ∧ [Γc ; γ ; {c₁} ⊢〚e〛σ ⇓ {c₂}] *)
+          nraenv_core_sem_select e env (d1::c1) c2              (**r ⇒ [Γc ; γ ; {d₁::c₁} ⊢〚e〛σ ⇓ {c₂}] *)
+      with nraenv_core_sem_map_env: nraenv_core -> list data -> data -> list data -> Prop :=
+      | sem_cNRAEnvMapEnv_empty : forall e d,
+          nraenv_core_sem_map_env e nil d nil                   (**r   [Γc ; {} ; d ⊢〚e〛χᵉ ⇓ {}] *)
+      | sem_cNRAEnvMapEnv_cons : forall e d1 d c1 d2 c2,
+          nraenv_core_sem e d1 d d2 ->                          (**r   [Γc ; d₁ ; d ⊢〚e〛⇓ d₂]  *)
+          nraenv_core_sem_map_env e c1 d c2 ->                  (**r ∧ [Γc ; {c₁} ; d ⊢〚e〛χᵉ ⇓ {c₂}] *)
+          nraenv_core_sem_map_env e (d1::c1) d (d2::c2)         (**r ⇒ [Γc ; {d₁::c₁} ; d ⊢〚e〛χᵉ ⇓ {d₂::c₂}] *)
+      .
+
+    End Denotation.
+
+    Section Evaluation.
+
+      Fixpoint nraenv_core_eval (e:nraenv_core) (envin: data) (din:data) : option data :=
+        match e with
+        | cNRAEnvGetConstant s =>
+          edot constant_env s
+        | cNRAEnvID =>
+          Some din
+        | cNRAEnvConst rd =>
+          Some (normalize_data h rd)
+        | cNRAEnvBinop bop e1 e2 =>
+          olift2 (fun d1 d2 => binary_op_eval h bop d1 d2)
+                 (nraenv_core_eval e1 envin din) (nraenv_core_eval e2 envin din)
+        | cNRAEnvUnop uop e =>
+          olift (fun d1 => unary_op_eval h uop d1)
+                (nraenv_core_eval e envin din)
+        | cNRAEnvMap e2 e1 =>
+          let aux_map d :=
+              lift_oncoll
+                (fun c1 => lift dcoll (lift_map (nraenv_core_eval e2 envin) c1)) d
+          in olift aux_map (nraenv_core_eval e1 envin din)
+        | cNRAEnvMapProduct e2 e1 =>
+          let aux_mapconcat d :=
+              lift_oncoll
+                (fun c1 => lift dcoll (omap_product (nraenv_core_eval e2 envin) c1)) d
+          in olift aux_mapconcat (nraenv_core_eval e1 envin din)
+        | cNRAEnvProduct e1 e2 =>
           (* Note: (fun y => nra_eval op2 x) does not depend on input,
              but we still use a nested loop and delay op2 evaluation
              so it does not fail in case the op1 operand is an empty
              collection -- this makes sure to align the semantics with
              the NNRC version. - Jerome *)
           let aux_product d :=
-              lift_oncoll (fun c1 => lift dcoll (omap_product (fun _ => nraenv_core_eval op2 env x) c1)) d
-          in olift aux_product (nraenv_core_eval op1 env x)
-      | cNRAEnvSelect op1 op2 =>
-        let pred x' :=
-            match nraenv_core_eval op1 env x' with
+              lift_oncoll
+                (fun c1 => lift dcoll (omap_product (fun _ => nraenv_core_eval e2 envin din) c1)) d
+          in olift aux_product (nraenv_core_eval e1 envin din)
+        | cNRAEnvSelect e2 e1 =>
+          let pred d1 :=
+              match nraenv_core_eval e2 envin d1 with
               | Some (dbool b) => Some b
               | _ => None
-            end
-        in
-        let aux_select d :=
-            lift_oncoll (fun c1 => lift dcoll (lift_filter pred c1)) d
-        in
-        olift aux_select (nraenv_core_eval op2 env x)
-      | cNRAEnvEither opl opr =>
-        match x with
-          | dleft dl => nraenv_core_eval opl env dl
-          | dright dr => nraenv_core_eval opr env dr
+              end
+          in
+          let aux_select d :=
+              lift_oncoll (fun d1 => lift dcoll (lift_filter pred d1)) d
+          in
+          olift aux_select (nraenv_core_eval e1 envin din)
+        | cNRAEnvDefault e1 e2 =>
+          olift (fun d1 =>
+                   match d1 with
+                   | dcoll nil => nraenv_core_eval e2 envin din
+                   | _ => Some d1
+                   end)
+                (nraenv_core_eval e1 envin din)
+        | cNRAEnvEither e1 e2 =>
+          match din with
+          | dleft d1 => nraenv_core_eval e1 envin d1
+          | dright d2 => nraenv_core_eval e2 envin d2
           | _ => None
-        end
-      | cNRAEnvEitherConcat op1 op2 =>
-        match nraenv_core_eval op1 env x, nraenv_core_eval op2 env x with
+          end
+        | cNRAEnvEitherConcat e1 e2 =>
+          match nraenv_core_eval e1 envin din, nraenv_core_eval e2 envin din with
           | Some (dleft (drec l)), Some (drec t)  =>
             Some (dleft (drec (rec_concat_sort l t)))
           | Some (dright (drec r)), Some (drec t)  =>
             Some (dright (drec (rec_concat_sort r t)))
           | _, _ => None
-        end
-      | cNRAEnvDefault op1 op2 =>
-        olift (fun d1 => match d1 with
-                               | dcoll nil => nraenv_core_eval op2 env x
-                               | _ => Some d1
-                         end) (nraenv_core_eval op1 env x)
-      | cNRAEnvApp op2 op1 =>
-        olift (fun x' => nraenv_core_eval op2 env x') (nraenv_core_eval op1 env x)
-      | cNRAEnvGetConstant s => edot constant_env s
-      | cNRAEnvEnv => (Some env)
-      | cNRAEnvAppEnv op2 op1 =>
-        (* Note: evaluate op1 to create a new environment;
-                 evaluate op2 in that new environment *)
-        (* This is the parallel to AApp, but for the environment *)
-        olift (fun env' => nraenv_core_eval op2 env' x) (nraenv_core_eval op1 env x)
-      | cNRAEnvMapEnv op1 =>
-        lift_oncoll (fun c1 => lift dcoll (lift_map ((fun env' => nraenv_core_eval op1 env' x)) c1)) env
-    end.
+          end
+        | cNRAEnvApp e2 e1 =>
+          olift (fun d1 => nraenv_core_eval e2 envin d1) (nraenv_core_eval e1 envin din)
+        | cNRAEnvEnv =>
+          Some envin
+        | cNRAEnvAppEnv e2 e1 =>
+          olift (fun env1 => nraenv_core_eval e2 env1 din) (nraenv_core_eval e1 envin din)
+        | cNRAEnvMapEnv e =>
+          lift_oncoll
+            (fun c1 => lift dcoll
+                            (lift_map ((fun env1 => nraenv_core_eval e env1 din)) c1)) envin
+        end.
 
-  (** Functions used to map dual input env/data into single input *)
-  (* Input encoding *)
+    End Evaluation.
 
-  Require Import NRARuntime.
+    Section EvalCorrect.
+      (** Auxiliary correctness lemmas for map, map_product, select and map_env judgments. *)
+      Lemma nraenv_core_eval_map_correct : forall e env l1 l2,
+        (forall env d1 d2 : data,
+            nraenv_core_eval e env d1 = Some d2 -> nraenv_core_sem e env d1 d2) ->
+        lift_map (nraenv_core_eval e env) l1 = Some l2 ->
+        nraenv_core_sem_map e env l1 l2.
+      Proof.
+        intros.
+        revert l2 H0.
+        induction l1; simpl in *; intros.
+        - inversion H0; econstructor.
+        - case_eq (nraenv_core_eval e env a); intros; rewrite H1 in *; [|congruence].
+          unfold lift in H0.
+          case_eq (lift_map (nraenv_core_eval e env) l1); intros; rewrite H2 in *; [|congruence].
+          specialize (IHl1 l eq_refl).
+          inversion H0.
+          econstructor; eauto.
+      Qed.
+          
+      Lemma nraenv_core_eval_map_product_correct : forall e env l1 l2,
+        (forall env d1 d2 : data,
+            nraenv_core_eval e env d1 = Some d2 -> nraenv_core_sem e env d1 d2) ->
+        omap_product (nraenv_core_eval e env) l1 = Some l2 ->
+        nraenv_core_sem_map_product e env l1 l2.
+      Proof.
+        intros.
+        revert l2 H0.
+        induction l1; simpl in *; intros.
+        - inversion H0; econstructor.
+        - generalize (omap_product_cons_inv (nraenv_core_eval e env) l1 a l2 H0); intros.
+          elim H1; clear H1; intros.
+          elim H1; clear H1; intros.
+          elim H1; clear H1; intros.
+          elim H2; clear H2; intros.
+          subst.
+          unfold oncoll_map_concat in H1.
+          case_eq (nraenv_core_eval e env a); intros; rewrite H3 in *; [|congruence].
+          case_eq d; intros; rewrite H4 in H1; try congruence.
+          subst.
+          specialize (H env a (dcoll l) H3).
+          rewrite omap_concat_correct_and_complete in H1.
+          apply (sem_cNRAEnvMapProduct_cons e env a l1 x0 l x).
+          + assumption.
+          + assumption.
+          + apply IHl1; assumption.
+      Qed.
+
+      Lemma nraenv_core_eval_select_correct e env l1 l2 :
+        (forall env d1 d2 : data,
+            nraenv_core_eval e env d1 = Some d2 -> nraenv_core_sem e env d1 d2) ->
+        lift_filter
+          (fun d1 : data =>
+             match nraenv_core_eval e env d1 with
+             | Some dunit => None
+             | Some (dnat _) => None
+             | Some (dbool b) => Some b
+             | Some (dstring _) => None
+             | Some (dcoll _) => None
+             | Some (drec _) => None
+             | Some (dleft _) => None
+             | Some (dright _) => None
+             | Some (dbrand _ _) => None
+             | Some (dforeign _) => None
+             | None => None
+             end) l1 = Some l2 ->
+        nraenv_core_sem_select e env l1 l2.
+      Proof.
+        intro.
+        revert l2; induction l1; simpl; intros.
+        - inversion H0. econstructor.
+        - case_eq (nraenv_core_eval e env a); intros; rewrite H1 in *; simpl in *.
+          destruct d; simpl in *; try congruence.
+          case_eq
+            (lift_filter
+               (fun d1 : data =>
+                  match nraenv_core_eval e env d1 with
+                  | Some dunit => None
+                  | Some (dnat _) => None
+                  | Some (dbool b) => Some b
+                  | Some (dstring _) => None
+                  | Some (dcoll _) => None
+                  | Some (drec _) => None
+                  | Some (dleft _) => None
+                  | Some (dright _) => None
+                  | Some (dbrand _ _) => None
+                  | Some (dforeign _) => None
+                  | None => None
+                  end) l1);
+            intros; rewrite H2 in *; clear H2; [|congruence].
+          specialize (IHl1 l eq_refl).
+          destruct b; simpl in *;
+            simpl in *; inversion H0; clear H0; subst.
+          + econstructor; eauto.
+          + econstructor; eauto.
+          + congruence.
+      Qed.
+
+      Lemma omap_product_some_is_oproduct d1 d2 l1 l2 :
+        omap_product (fun _ : data => Some d2) (d1 :: l1) = Some l2 ->
+        exists l, d2 = dcoll l /\ oproduct (d1::l1) l = Some l2.
+      Proof.
+        intros.
+        unfold omap_product, oproduct in *; simpl in *.
+        case_eq d2; intros; rewrite H0 in *; simpl in *; try congruence.
+        exists l; split; [reflexivity| ].
+        unfold oncoll_map_concat in H.
+        destruct (omap_concat d1 l); [|congruence].
+        assumption.
+      Qed.
+
+      Lemma nraenv_core_eval_map_env_correct : forall e l1 d l2,
+        (forall env d1 d2 : data,
+            nraenv_core_eval e env d1 = Some d2 -> nraenv_core_sem e env d1 d2) ->
+        lift_map (fun env1 : data => nraenv_core_eval e env1 d) l1 = Some l2 ->
+        nraenv_core_sem_map_env e l1 d l2.
+      Proof.
+        intros.
+        revert l2 H0.
+        induction l1; simpl in *; intros.
+        - inversion H0; econstructor.
+        - case_eq (nraenv_core_eval e a d); intros; rewrite H1 in *; [|congruence].
+          unfold lift in H0.
+          case_eq (lift_map (fun env1 : data => nraenv_core_eval e env1 d) l1);
+            intros; rewrite H2 in *; [|congruence].
+          specialize (IHl1 l eq_refl).
+          inversion H0.
+          econstructor; eauto.
+      Qed.
+
+      (** Evaluation is correct wrt. the cNRAEnv semantics. *)
+
+      Lemma nraenv_core_eval_correct : forall e env d1 d2,
+          nraenv_core_eval e env d1 = Some d2 ->
+          nraenv_core_sem e env d1 d2.
+      Proof.
+        induction e; simpl; intros.
+        - econstructor; eauto.
+        - inversion H; econstructor; eauto.
+        - inversion H; econstructor; eauto.
+        - unfold olift2 in H.
+          case_eq (nraenv_core_eval e1 env d1); intros; rewrite H0 in *; [|congruence].
+          case_eq (nraenv_core_eval e2 env d1); intros; rewrite H1 in *; [|congruence].
+          specialize (IHe1 env d1 d H0); specialize (IHe2 env d1 d0 H1);
+            econstructor; eauto.
+        - unfold olift in H.
+          case_eq (nraenv_core_eval e env d1); intros; rewrite H0 in *; [|congruence].
+          specialize (IHe env d1 d H0); econstructor; eauto.
+        - unfold olift in H.
+          case_eq (nraenv_core_eval e2 env d1); intros; rewrite H0 in *; [|congruence].
+          unfold lift_oncoll in H.
+          destruct d; simpl in H; try congruence.
+          unfold lift in H.
+          case_eq (lift_map (nraenv_core_eval e1 env) l); intros; rewrite H1 in *; [|congruence].
+          inversion H; subst; clear H.
+          econstructor; eauto.
+          apply nraenv_core_eval_map_correct; auto.
+        - unfold olift in H.
+          case_eq (nraenv_core_eval e2 env d1); intros; rewrite H0 in *; [|congruence].
+          unfold lift_oncoll in H.
+          destruct d; simpl in H; try congruence.
+          unfold lift in H.
+          case_eq (omap_product (nraenv_core_eval e1 env) l); intros; rewrite H1 in *; [|congruence].
+          inversion H; subst; clear H.
+          econstructor; eauto.
+          apply nraenv_core_eval_map_product_correct; auto.
+        - unfold olift2 in H.
+          case_eq (nraenv_core_eval e1 env d1); intros; rewrite H0 in *; simpl in *; [|congruence].
+          destruct d; simpl in *; try congruence.
+          destruct l; simpl in *.
+          (* Left collection is empty *)
+          + inversion H; subst.
+            econstructor; eauto.
+          (* Left collection is not empty *)
+          + specialize (IHe1 env d1 (dcoll (d::l)) H0).
+            unfold lift in H.
+            case_eq (nraenv_core_eval e2 env d1); intros; rewrite H1 in *.
+            * case_eq (omap_product (fun _ : data => nraenv_core_eval e2 env d1) (d :: l)); intros;
+                rewrite H1 in H2; simpl in *; rewrite H2 in *; [|congruence].
+              inversion H; clear H; subst.
+              elim (omap_product_some_is_oproduct d d0 l l0 H2); intros.
+              elim H; clear H; intros; subst.
+              econstructor; eauto. congruence.
+              apply oproduct_correct; assumption.
+            * unfold omap_product in H; simpl in H.
+              congruence.
+        - unfold olift in H.
+          case_eq (nraenv_core_eval e2 env d1); intros; rewrite H0 in *; [|congruence].
+          unfold lift_oncoll in H.
+          destruct d; simpl in H; try congruence.
+          unfold lift in H.
+          specialize (IHe2 env d1 (dcoll l) H0).
+          case_eq
+            (lift_filter
+               (fun d1 : data =>
+                  match nraenv_core_eval e1 env d1 with
+                  | Some dunit => None
+                  | Some (dnat _) => None
+                  | Some (dbool b) => Some b
+                  | Some (dstring _) => None
+                  | Some (dcoll _) => None
+                  | Some (drec _) => None
+                  | Some (dleft _) => None
+                  | Some (dright _) => None
+                  | Some (dbrand _ _) => None
+                  | Some (dforeign _) => None
+                  | None => None
+                  end) l); intros; rewrite H1 in *; [|congruence].
+          inversion H; clear H; subst.
+          econstructor; eauto.
+          apply nraenv_core_eval_select_correct; auto.
+        - unfold olift in H.
+          case_eq (nraenv_core_eval e1 env d1); intros; rewrite H0 in *; [|congruence].
+          elim (data_eq_dec d (dcoll nil)); intros.
+          subst.
+          + econstructor; eauto.
+          + destruct d; inversion H; subst; auto;
+              eapply sem_cNRAEnvDefault_not_empty; auto;
+                destruct l; auto; inversion H; subst; auto.
+            congruence.
+        - destruct d1; try congruence.
+          econstructor; apply IHe1; auto.
+          econstructor; apply IHe2; auto.
+        - case_eq (nraenv_core_eval e1 env d1); intros; rewrite H0 in *; [|congruence].
+          destruct d; intros; try congruence.
+         + destruct d; intros; try congruence.
+           case_eq (nraenv_core_eval e2 env d1); intros; rewrite H1 in *; [|congruence].
+           destruct d; intros; try congruence.
+           inversion H; subst; clear H; intros.
+           econstructor; eauto.
+         + destruct d; intros; try congruence.
+           case_eq (nraenv_core_eval e2 env d1); intros; rewrite H1 in *; [|congruence].
+           destruct d; intros; try congruence.
+           inversion H; subst; clear H; intros.
+           econstructor; eauto.
+        - unfold olift in H.
+          case_eq (nraenv_core_eval e2 env d1); intros; rewrite H0 in *; [|congruence].
+          econstructor; eauto.
+        - inversion H; subst; econstructor.
+        - unfold olift in H.
+          case_eq (nraenv_core_eval e2 env d1); intros; rewrite H0 in *; [|congruence].
+          econstructor; eauto.
+        - unfold lift_oncoll in H.
+          destruct env; simpl in H; try congruence.
+          unfold lift in H.
+          case_eq (lift_map (fun env1 : data => nraenv_core_eval e env1 d1) l);
+            intros; rewrite H0 in *; [|congruence].
+          inversion H; subst; clear H.
+          econstructor; eauto.
+          apply nraenv_core_eval_map_env_correct; auto.
+      Qed.
+ 
+      (** Auxiliary lemmas used in the completeness theorem *)
+
+      Lemma nraenv_core_map_eval_complete e env c1 c2:
+        (forall env d1 d2 : data,
+            nraenv_core_sem e env d1 d2 -> nraenv_core_eval e env d1 = Some d2) ->
+        (nraenv_core_sem_map e env c1 c2) ->
+        lift dcoll (lift_map (nraenv_core_eval e env) c1) = Some (dcoll c2).
+      Proof.
+        intros.
+        revert c2 H0.
+        induction c1; simpl in *; intros.
+        - inversion H0; reflexivity.
+        - inversion H0; clear H0; subst.
+          rewrite (H env a d2 H5); simpl.
+          specialize (IHc1 c3 H7).
+          unfold lift in *.
+          case_eq (lift_map (nraenv_core_eval e env) c1); intros; rewrite H0 in *; [|congruence].
+          inversion IHc1; clear IHc1; subst; reflexivity.
+      Qed.
+
+      Lemma nraenv_core_map_product_eval_complete e env c1 c2:
+        (forall env d1 d2 : data,
+            nraenv_core_sem e env d1 d2 -> nraenv_core_eval e env d1 = Some d2) ->
+        (nraenv_core_sem_map_product e env c1 c2) ->
+        lift dcoll (omap_product (nraenv_core_eval e env) c1) = Some (dcoll c2).
+      Proof.
+        intros.
+        revert c2 H0.
+        induction c1; simpl in *; intros.
+        - inversion H0; reflexivity.
+        - inversion H0; clear H0; subst.
+          unfold omap_product in *.
+          unfold oncoll_map_concat in *; simpl.
+          rewrite (H env a (dcoll c4) H3); simpl.
+          rewrite <- omap_concat_correct_and_complete in H6.
+          rewrite H6; simpl.
+          specialize (IHc1 c3 H8).
+          unfold lift in *.
+          destruct (lift_flat_map
+             (fun a : data =>
+              match nraenv_core_eval e env a with
+              | Some dunit => None
+              | Some (dnat _) => None
+              | Some (dbool _) => None
+              | Some (dstring _) => None
+              | Some (dcoll y) => omap_concat a y
+              | Some (drec _) => None
+              | Some (dleft _) => None
+              | Some (dright _) => None
+              | Some (dbrand _ _) => None
+              | Some (dforeign _) => None
+              | None => None
+              end) c1); [|congruence].
+          inversion IHc1; reflexivity.
+      Qed.
+        
+      Lemma nraenv_core_select_eval_complete e env c1 c2:
+        (forall env d1 d2 : data,
+            nraenv_core_sem e env d1 d2 -> nraenv_core_eval e env d1 = Some d2) ->
+        (nraenv_core_sem_select e env c1 c2) ->
+        lift dcoll
+             (lift_filter
+                (fun d0 : data =>
+                   match nraenv_core_eval e env d0 with
+                   | Some dunit => None
+                   | Some (dnat _) => None
+                   | Some (dbool b) => Some b
+                   | Some (dstring _) => None
+                   | Some (dcoll _) => None
+                   | Some (drec _) => None
+                   | Some (dleft _) => None
+                   | Some (dright _) => None
+                   | Some (dbrand _ _) => None
+                   | Some (dforeign _) => None
+                   | None => None
+                   end) c1) = Some (dcoll c2).
+      Proof.
+        intros.
+        revert c2 H0.
+        induction c1; simpl in *; intros.
+        - inversion H0; reflexivity.
+        - inversion H0; clear H0; subst.
+          (* condition is true *)
+          + rewrite (H env a (dbool true) H5); simpl.
+            specialize (IHc1 c3 H7).
+            destruct
+              (lift_filter
+                 (fun d0 : data =>
+                    match nraenv_core_eval e env d0 with
+                    | Some dunit => None
+                    | Some (dnat _) => None
+                    | Some (dbool b) => Some b
+                    | Some (dstring _) => None
+                    | Some (dcoll _) => None
+                    | Some (drec _) => None
+                    | Some (dleft _) => None
+                    | Some (dright _) => None
+                    | Some (dbrand _ _) => None
+                    | Some (dforeign _) => None
+                    | None => None
+                    end) c1); simpl in *; [|congruence].
+            inversion IHc1; reflexivity.
+          + rewrite (H env a (dbool false) H5); simpl.
+            specialize (IHc1 c2 H7).
+            destruct
+              (lift_filter
+                 (fun d0 : data =>
+                    match nraenv_core_eval e env d0 with
+                    | Some dunit => None
+                    | Some (dnat _) => None
+                    | Some (dbool b) => Some b
+                    | Some (dstring _) => None
+                    | Some (dcoll _) => None
+                    | Some (drec _) => None
+                    | Some (dleft _) => None
+                    | Some (dright _) => None
+                    | Some (dbrand _ _) => None
+                    | Some (dforeign _) => None
+                    | None => None
+                    end) c1); simpl in *; [|congruence].
+            inversion IHc1; reflexivity.
+      Qed.
+
+      Lemma nraenv_core_map_env_eval_complete e c1 d c2:
+        (forall env d1 d2 : data,
+            nraenv_core_sem e env d1 d2 -> nraenv_core_eval e env d1 = Some d2) ->
+        (nraenv_core_sem_map_env e c1 d c2) ->
+        lift dcoll (lift_map (fun env1 : data => nraenv_core_eval e env1 d) c1) = Some (dcoll c2).
+      Proof.
+        intros.
+        revert c2 H0.
+        induction c1; simpl in *; intros.
+        - inversion H0; reflexivity.
+        - inversion H0; clear H0; subst.
+          rewrite (H a d d2 H4); simpl.
+          specialize (IHc1 c3 H7).
+          unfold lift in *.
+          case_eq (lift_map (fun env1 : data => nraenv_core_eval e env1 d) c1);
+            intros; rewrite H0 in *; [|congruence].
+          inversion IHc1; clear IHc1; subst; reflexivity.
+      Qed.
+
+      (** Evaluation is complete wrt. the cNRAEnv semantics. *)
+
+      Lemma nraenv_core_eval_complete : forall e env d1 d2,
+          nraenv_core_sem e env d1 d2 ->
+          nraenv_core_eval e env d1 = Some d2.
+      Proof.
+        induction e; intros.
+        - inversion H; subst; simpl; auto.
+        - inversion H; subst; simpl; auto.
+        - inversion H; subst; simpl; auto.
+        - inversion H; subst; simpl.
+          rewrite (IHe1 env d1 d0 H3);
+            rewrite (IHe2 env d1 d3 H7); simpl; auto.
+        - inversion H; subst; simpl.
+          rewrite (IHe env d1 d0 H2); simpl; auto.
+        - inversion H; subst; simpl.
+          rewrite (IHe2 env d1 (dcoll c1) H2); simpl.
+          apply nraenv_core_map_eval_complete; auto.
+        - inversion H; subst; simpl.
+          rewrite (IHe2 env d1 (dcoll c1) H2); simpl.
+          apply nraenv_core_map_product_eval_complete; auto.
+        - inversion H; subst; simpl.
+          (* empty first collection *)
+          + rewrite (IHe1 env d1 (dcoll nil) H5); reflexivity.
+          + destruct c1; [congruence| ]; clear H3.
+            rewrite (IHe1 env d1 (dcoll (d :: c1)) H2); simpl.
+            rewrite <- oproduct_correct_and_complete in H8.
+            rewrite (IHe2 env d1 (dcoll c2) H4).
+            unfold oproduct in H8.
+            unfold omap_product.
+            unfold oncoll_map_concat.
+            unfold omap_concat in *.
+            rewrite H8; reflexivity.
+        - inversion H; subst; simpl.
+          rewrite (IHe2 env d1 (dcoll c1) H2); simpl.
+          apply nraenv_core_select_eval_complete; auto.
+        - inversion H; subst; simpl.
+          (* empty collection case *)
+          + rewrite (IHe1 env d1 (dcoll nil) H2); simpl; auto.
+          (* non-empty collection case *)
+          + rewrite (IHe1 env d1 d2 H2); simpl; auto.
+            destruct d2; try congruence.
+            destruct l; congruence.
+        - inversion H; subst; simpl; auto.
+        - inversion H; subst; simpl.
+          (* left case *)
+          + rewrite (IHe1 env d1 (dleft (drec r1)) H2); simpl.
+            rewrite (IHe2 env d1 (drec r2) H6); reflexivity.
+          (* right case *)
+          + rewrite (IHe1 env d1 (dright (drec r1)) H2); simpl.
+            rewrite (IHe2 env d1 (drec r2) H6); reflexivity.
+        - inversion H; subst; simpl.
+          rewrite (IHe2 env d1 d0 H2); simpl.
+          rewrite (IHe1 env d0 d2 H6); reflexivity.
+        - inversion H; subst; simpl; auto.
+        - inversion H; subst; simpl.
+          rewrite (IHe2 env d1 env1 H2); simpl.
+          rewrite (IHe1 env1 d1 d2 H6); reflexivity.
+        - inversion H; subst; simpl.
+          apply nraenv_core_map_env_eval_complete; auto.
+      Qed.
+
+      (** Main equivalence theorem. *)
+      
+      Theorem nraenv_core_eval_correct_and_complete : forall e env d d',
+          nraenv_core_eval e env d = Some d' <-> nraenv_core_sem e env d d'.
+      Proof.
+        split.
+        apply nraenv_core_eval_correct.
+        apply nraenv_core_eval_complete.
+      Qed.
+
+    End EvalCorrect.
+
+    (** Functions used to map dual input env/data into single input *)
+    (* Input encoding *)
+
+    Require Import NRARuntime.
   
-  Local Open Scope string_scope.
-  Local Open Scope list_scope.
+    Local Open Scope string_scope.
+    Local Open Scope list_scope.
 
-  Definition NRARecEither f :=
-    NRAEither (NRAUnop OpLeft (NRAUnop (OpRec f) NRAID))
-              (NRAUnop OpRight (NRAUnop (OpRec f) NRAID)).
+    Definition NRARecEither f :=
+      NRAEither (NRAUnop OpLeft (NRAUnop (OpRec f) NRAID))
+                (NRAUnop OpRight (NRAUnop (OpRec f) NRAID)).
   
-  Fixpoint nra_of_nraenv_core (ae:nraenv_core) : nra :=
-    match ae with
-    | cNRAEnvID =>
-      nra_data
-    | cNRAEnvConst d =>
-      NRAConst d
-    | cNRAEnvBinop b ae1 ae2 =>
-      NRABinop b (nra_of_nraenv_core ae1) (nra_of_nraenv_core ae2)
-    | cNRAEnvUnop u ae1 =>
-      NRAUnop u (nra_of_nraenv_core ae1)
-    | cNRAEnvMap ea1 ea2 =>
-      NRAMap (nra_of_nraenv_core ea1)
-             (unnest_two
-                "a1"
-                "PDATA"
-                (NRAUnop OpBag (nra_wrap_a1 (nra_of_nraenv_core ea2))))
-    | cNRAEnvMapProduct ea1 ea2 =>
-      (NRAMap (NRABinop OpRecConcat
-                        (NRAUnop (OpDot "PDATA") NRAID)
-                        (NRAUnop (OpDot "PDATA2") NRAID))
-              (NRAMapProduct
-                 (NRAMap (NRAUnop (OpRec "PDATA2") NRAID) (nra_of_nraenv_core ea1))
-                 (unnest_two
-                    "a1"
-                    "PDATA"
-                    (NRAUnop OpBag (nra_wrap_a1 (nra_of_nraenv_core ea2))))))
-    | cNRAEnvProduct ea1 ea2 =>
-      NRAProduct (nra_of_nraenv_core ea1) (nra_of_nraenv_core ea2)
-    | cNRAEnvSelect ea1 ea2 =>
-      (NRAMap (NRAUnop (OpDot "PDATA") NRAID)
-              (NRASelect (nra_of_nraenv_core ea1)
-                         (unnest_two
-                            "a1"
-                            "PDATA"
-                            (NRAUnop OpBag (nra_wrap_a1 (nra_of_nraenv_core ea2))))))
-    | cNRAEnvDefault ea1 ea2 =>
-      NRADefault (nra_of_nraenv_core ea1) (nra_of_nraenv_core ea2)
-    | cNRAEnvEither eal ear =>
-      NRAApp
-        (NRAEither (nra_of_nraenv_core eal) (nra_of_nraenv_core ear))
-        (NRAEitherConcat
-           (NRAApp (NRARecEither "PDATA") nra_data)
-           (NRAUnop (OpRec "PBIND") nra_bind))
-    | cNRAEnvEitherConcat ea1 ea2 =>
-      NRAEitherConcat (nra_of_nraenv_core ea1) (nra_of_nraenv_core ea2)
-    | cNRAEnvApp ea1 ea2 =>
-      NRAApp (nra_of_nraenv_core ea1)
-             (nra_wrap (nra_of_nraenv_core ea2))
-    | cNRAEnvGetConstant s =>
-      NRAGetConstant s
-    | cNRAEnvEnv => nra_bind
-    | cNRAEnvAppEnv ea1 ea2 =>
-      NRAApp (nra_of_nraenv_core ea1)
-             (nra_context (nra_of_nraenv_core ea2) nra_data)
-    | cNRAEnvMapEnv ea1 =>
-      (* fix this: the nra_data should change to a nra_pair *)
-      NRAMap (nra_of_nraenv_core ea1)
-             (unnest_two
-                "a1"
-                "PBIND"
-                (NRAUnop OpBag (nra_wrap_bind_a1 nra_data)))
-    end.
+    Fixpoint nra_of_nraenv_core (ae:nraenv_core) : nra :=
+      match ae with
+      | cNRAEnvGetConstant s =>
+        NRAGetConstant s
+      | cNRAEnvID =>
+        nra_data
+      | cNRAEnvConst d =>
+        NRAConst d
+      | cNRAEnvBinop b ae1 ae2 =>
+        NRABinop b (nra_of_nraenv_core ae1) (nra_of_nraenv_core ae2)
+      | cNRAEnvUnop u ae1 =>
+        NRAUnop u (nra_of_nraenv_core ae1)
+      | cNRAEnvMap ea1 ea2 =>
+        NRAMap (nra_of_nraenv_core ea1)
+               (unnest_two
+                  "a1"
+                  "PDATA"
+                  (NRAUnop OpBag (nra_wrap_a1 (nra_of_nraenv_core ea2))))
+      | cNRAEnvMapProduct ea1 ea2 =>
+        (NRAMap (NRABinop OpRecConcat
+                          (NRAUnop (OpDot "PDATA") NRAID)
+                          (NRAUnop (OpDot "PDATA2") NRAID))
+                (NRAMapProduct
+                   (NRAMap (NRAUnop (OpRec "PDATA2") NRAID) (nra_of_nraenv_core ea1))
+                   (unnest_two
+                      "a1"
+                      "PDATA"
+                      (NRAUnop OpBag (nra_wrap_a1 (nra_of_nraenv_core ea2))))))
+      | cNRAEnvProduct ea1 ea2 =>
+        NRAProduct (nra_of_nraenv_core ea1) (nra_of_nraenv_core ea2)
+      | cNRAEnvSelect ea1 ea2 =>
+        (NRAMap (NRAUnop (OpDot "PDATA") NRAID)
+                (NRASelect (nra_of_nraenv_core ea1)
+                           (unnest_two
+                              "a1"
+                              "PDATA"
+                              (NRAUnop OpBag (nra_wrap_a1 (nra_of_nraenv_core ea2))))))
+      | cNRAEnvDefault ea1 ea2 =>
+        NRADefault (nra_of_nraenv_core ea1) (nra_of_nraenv_core ea2)
+      | cNRAEnvEither eal ear =>
+        NRAApp
+          (NRAEither (nra_of_nraenv_core eal) (nra_of_nraenv_core ear))
+          (NRAEitherConcat
+             (NRAApp (NRARecEither "PDATA") nra_data)
+             (NRAUnop (OpRec "PBIND") nra_bind))
+      | cNRAEnvEitherConcat ea1 ea2 =>
+        NRAEitherConcat (nra_of_nraenv_core ea1) (nra_of_nraenv_core ea2)
+      | cNRAEnvApp ea1 ea2 =>
+        NRAApp (nra_of_nraenv_core ea1)
+               (nra_wrap (nra_of_nraenv_core ea2))
+      | cNRAEnvEnv => nra_bind
+      | cNRAEnvAppEnv ea1 ea2 =>
+        NRAApp (nra_of_nraenv_core ea1)
+               (nra_context (nra_of_nraenv_core ea2) nra_data)
+      | cNRAEnvMapEnv ea1 =>
+        (* fix this: the nra_data should change to a nra_pair *)
+        NRAMap (nra_of_nraenv_core ea1)
+               (unnest_two
+                  "a1"
+                  "PBIND"
+                  (NRAUnop OpBag (nra_wrap_bind_a1 nra_data)))
+      end.
 
-  Lemma lift_map_map_rec1 l s:
-    lift_map (fun x : data => Some (drec ((s, x) :: nil))) l =
-    Some (map (fun x : data => (drec ((s, x) :: nil))) l).
-  Proof.
-    induction l; try reflexivity; simpl; rewrite IHl; reflexivity.
-  Qed.
-
-  Lemma lift_map_map_rec2 env a1 l :
-    (lift_map
-       (fun x : data =>
-          match x with
+    Lemma lift_map_map_rec1 l s:
+      lift_map (fun x : data => Some (drec ((s, x) :: nil))) l =
+      Some (map (fun x : data => (drec ((s, x) :: nil))) l).
+    Proof.
+      induction l; try reflexivity; simpl; rewrite IHl; reflexivity.
+    Qed.
+    
+    Lemma lift_map_map_rec2 env a1 l :
+      (lift_map
+         (fun x : data =>
+            match x with
             | drec r1 =>
               Some
                 (drec
                    (rec_concat_sort
                       (("PBIND", env) :: ("a1", dcoll a1) :: nil) r1))
             | _  => None
-          end)
-       (map (fun x : data => drec (("PDATA", x) :: nil)) l))
-    =
-    Some (map (fun x : data =>  drec (("PBIND", env) :: ("PDATA", x) :: ("a1", dcoll a1) :: nil)) l).
-  Proof.
-    induction l; try reflexivity; simpl.
-    rewrite IHl; reflexivity.
-  Qed.
+            end)
+         (map (fun x : data => drec (("PDATA", x) :: nil)) l))
+      =
+      Some (map (fun x : data =>  drec (("PBIND", env) :: ("PDATA", x) :: ("a1", dcoll a1) :: nil)) l).
+    Proof.
+      induction l; try reflexivity; simpl.
+      rewrite IHl; reflexivity.
+    Qed.
 
-  Lemma lift_map_map_rec3 d a1 l :
-    (lift_map
-       (fun x : data =>
-          match x with
+    Lemma lift_map_map_rec3 d a1 l :
+      (lift_map
+         (fun x : data =>
+            match x with
             | drec r1 =>
               Some
                 (drec
                    (rec_concat_sort
                       (("PDATA", d) :: ("a1", dcoll a1) :: nil) r1))
             | _ => None
-          end)
-       (map (fun x : data => drec (("PBIND", x) :: nil)) l))
-    =
-    Some (map (fun x : data =>  drec (("PBIND", x) :: ("PDATA", d) :: ("a1", dcoll a1) :: nil)) l).
-  Proof.
-    induction l; try reflexivity; simpl.
-    rewrite IHl; reflexivity.
-  Qed.
+            end)
+         (map (fun x : data => drec (("PBIND", x) :: nil)) l))
+      =
+      Some (map (fun x : data =>  drec (("PBIND", x) :: ("PDATA", d) :: ("a1", dcoll a1) :: nil)) l).
+    Proof.
+      induction l; try reflexivity; simpl.
+      rewrite IHl; reflexivity.
+    Qed.
 
-  Lemma option_id {A} (x:option A) :
-    (match x with None => None | Some y => Some y end) = x.
-  Proof.
-    destruct x; reflexivity.
-  Qed.
+    Lemma option_id {A} (x:option A) :
+      (match x with None => None | Some y => Some y end) = x.
+    Proof.
+      destruct x; reflexivity.
+    Qed.
   
-  Lemma lift_map_map_unnest2 env a l0 l1 :
-    lift_map
-      (fun x : data =>
-         olift2
-           (fun d1 d2 : data =>
-              match d1 with
+    Lemma lift_map_map_unnest2 env a l0 l1 :
+      lift_map
+        (fun x : data =>
+           olift2
+             (fun d1 d2 : data =>
+                match d1 with
                 | drec r1 =>
                   match d2 with
-                    | drec r2 => Some (drec (rec_sort (r1 ++ r2)))
-                    | _ => None
+                  | drec r2 => Some (drec (rec_sort (r1 ++ r2)))
+                  | _ => None
                   end
                 | _ => None
-              end)
-           match x with
+                end)
+             match x with
              | drec r => edot r "PDATA"
              | _ => None
-           end
-           match x with
+             end
+             match x with
              | drec r => edot r "PDATA2"
              | _ => None
-           end)
-      (map
-         (fun x : data =>
-            drec (("PBIND", env) :: ("PDATA", a) :: ("PDATA2", x) :: nil)) l0 ++ l1)
-    =
-    olift2 (fun d1 d2 => Some (d1 ++ d2))
-           (lift_map
-              (fun x : data =>
-                 match a with
+             end)
+        (map
+           (fun x : data =>
+              drec (("PBIND", env) :: ("PDATA", a) :: ("PDATA2", x) :: nil)) l0 ++ l1)
+      =
+      olift2 (fun d1 d2 => Some (d1 ++ d2))
+             (lift_map
+                (fun x : data =>
+                   match a with
                    | drec r2 =>
                      match x with
-                       | drec r1 => Some (drec (rec_concat_sort r2 r1))
-                       | _ => None
+                     | drec r1 => Some (drec (rec_concat_sort r2 r1))
+                     | _ => None
                      end
                    | _ => None
-                 end) l0)
-           (lift_map
-              (fun x : data =>
-                 olift2
-                   (fun d1 d2 : data =>
-                      match d1 with
+                   end) l0)
+             (lift_map
+                (fun x : data =>
+                   olift2
+                     (fun d1 d2 : data =>
+                        match d1 with
                         | drec r1 =>
                           match d2 with
-                            | drec r2 => Some (drec (rec_sort (r1 ++ r2)))
-                            | _ => None
+                          | drec r2 => Some (drec (rec_sort (r1 ++ r2)))
+                          | _ => None
                           end
                         | _ => None
-                      end)
-                   match x with
+                        end)
+                     match x with
                      | drec r => edot r "PDATA"
                      | _ => None
-                   end
-                   match x with
+                     end
+                     match x with
                      | drec r => edot r "PDATA2"
                      | _ => None
-                   end)
-              l1).
-  Proof.
-    induction l0; try reflexivity; simpl.
-    rewrite option_id; reflexivity.
-    rewrite IHl0; clear IHl0; simpl.
-    destruct a; try reflexivity.
-    destruct a0; try reflexivity.
-    simpl.
-    destruct ((lift_map
-           (fun x : data =>
-            match x with
-            | drec r1 => Some (drec (rec_concat_sort l r1))
-            | _ => None
-            end) l0)); try reflexivity; simpl.
-    generalize (     lift_map
-       (fun x : data =>
-        olift2
-          (fun d1 d2 : data =>
-           match d1 with
-           | drec r1 =>
-               match d2 with
-               | drec r2 => Some (drec (rec_sort (r1 ++ r2)))
-               | _ => None
-               end
-           | _ => None
-           end)
-          match x with
-          | drec r => edot r "PDATA"
-          | _ => None
-          end
-          match x with
-          | drec r => edot r "PDATA2"
-          | _ => None
-          end) l1); intros.
-    destruct o; reflexivity.
-  Qed.
+                     end)
+                l1).
+    Proof.
+      induction l0; try reflexivity; simpl.
+      rewrite option_id; reflexivity.
+      rewrite IHl0; clear IHl0; simpl.
+      destruct a; try reflexivity.
+      destruct a0; try reflexivity.
+      simpl.
+      destruct ((lift_map
+                   (fun x : data =>
+                      match x with
+                      | drec r1 => Some (drec (rec_concat_sort l r1))
+                      | _ => None
+                      end) l0)); try reflexivity; simpl.
+      generalize (     lift_map
+                         (fun x : data =>
+                            olift2
+                              (fun d1 d2 : data =>
+                                 match d1 with
+                                 | drec r1 =>
+                                   match d2 with
+                                   | drec r2 => Some (drec (rec_sort (r1 ++ r2)))
+                                   | _ => None
+                                   end
+                                 | _ => None
+                                 end)
+                              match x with
+                              | drec r => edot r "PDATA"
+                              | _ => None
+                              end
+                              match x with
+                              | drec r => edot r "PDATA2"
+                              | _ => None
+                              end) l1); intros.
+      destruct o; reflexivity.
+    Qed.
 
-  Lemma omap_concat_map_rec env a1 l :
-    omap_concat
-      (drec (("PBIND", env) :: ("a1", dcoll a1) :: nil))
-      (map (fun x : data => drec (("PDATA", x) :: nil)) l)
-    =
-    Some (map (fun x : data =>  drec (("PBIND", env) :: ("PDATA", x) :: ("a1", dcoll a1) :: nil)) l).
-  Proof.
-    unfold omap_concat; simpl.
-    induction l; try reflexivity; simpl.
-    rewrite IHl; reflexivity.
-  Qed.
+    Lemma omap_concat_map_rec env a1 l :
+      omap_concat
+        (drec (("PBIND", env) :: ("a1", dcoll a1) :: nil))
+        (map (fun x : data => drec (("PDATA", x) :: nil)) l)
+      =
+      Some (map (fun x : data =>  drec (("PBIND", env) :: ("PDATA", x) :: ("a1", dcoll a1) :: nil)) l).
+    Proof.
+      unfold omap_concat; simpl.
+      induction l; try reflexivity; simpl.
+      rewrite IHl; reflexivity.
+    Qed.
 
-  Lemma omap_concat_map_rec2 env a l :
-    omap_concat (drec (("PBIND", env) :: ("PDATA", a) :: nil))
-                (map (fun x : data => drec (("PDATA2", x) :: nil)) l)
+    Lemma omap_concat_map_rec2 env a l :
+      omap_concat (drec (("PBIND", env) :: ("PDATA", a) :: nil))
+                  (map (fun x : data => drec (("PDATA2", x) :: nil)) l)
+                  
+      =
+      Some (map (fun x : data =>  drec (("PBIND", env) :: ("PDATA", a) :: ("PDATA2", x) :: nil)) l).
+    Proof.
+      unfold omap_concat; simpl.
+      induction l; try reflexivity; simpl.
+      rewrite IHl; reflexivity.
+    Qed.
 
-    =
-    Some (map (fun x : data =>  drec (("PBIND", env) :: ("PDATA", a) :: ("PDATA2", x) :: nil)) l).
-  Proof.
-    unfold omap_concat; simpl.
-    induction l; try reflexivity; simpl.
-    rewrite IHl; reflexivity.
-  Qed.
+    Lemma omap_concat_map_rec3 d a1 l :
+      omap_concat
+        (drec (("PDATA", d) :: ("a1", dcoll a1) :: nil))
+        (map (fun x : data => drec (("PBIND", x) :: nil)) l)
+      =
+      Some (map (fun x : data =>  drec (("PBIND", x) :: ("PDATA", d) :: ("a1", dcoll a1) :: nil)) l).
+    Proof.
+      unfold omap_concat; simpl.
+      induction l; try reflexivity; simpl.
+      rewrite IHl; reflexivity.
+    Qed.
 
-  Lemma omap_concat_map_rec3 d a1 l :
-    omap_concat
-      (drec (("PDATA", d) :: ("a1", dcoll a1) :: nil))
-      (map (fun x : data => drec (("PBIND", x) :: nil)) l)
-    =
-    Some (map (fun x : data =>  drec (("PBIND", x) :: ("PDATA", d) :: ("a1", dcoll a1) :: nil)) l).
-  Proof.
-    unfold omap_concat; simpl.
-    induction l; try reflexivity; simpl.
-    rewrite IHl; reflexivity.
-  Qed.
+    Lemma omap_concat_unnest env a a1 l :
+      omap_concat
+        (drec (("PBIND", env) :: ("a1", dcoll a1) :: nil))
+        (drec (("PDATA", a) :: nil)
+              :: map (fun x : data => drec (("PDATA", x) :: nil)) l)
+      =
+      Some (drec (("PBIND", env) :: ("PDATA", a) :: ("a1", dcoll a1) :: nil) ::
+                 (map (fun x : data => drec (("PBIND", env) :: ("PDATA", x) :: ("a1", dcoll a1) :: nil)) l)).
+    Proof.
+      unfold omap_concat; simpl.
+      rewrite lift_map_map_rec2; simpl; reflexivity.
+    Qed.
 
-  Lemma omap_concat_unnest env a a1 l :
-    omap_concat
-      (drec (("PBIND", env) :: ("a1", dcoll a1) :: nil))
-      (drec (("PDATA", a) :: nil)
-            :: map (fun x : data => drec (("PDATA", x) :: nil)) l)
-    =
-    Some (drec (("PBIND", env) :: ("PDATA", a) :: ("a1", dcoll a1) :: nil) ::
-               (map (fun x : data => drec (("PBIND", env) :: ("PDATA", x) :: ("a1", dcoll a1) :: nil)) l)).
-  Proof.
-    unfold omap_concat; simpl.
-    rewrite lift_map_map_rec2; simpl; reflexivity.
-  Qed.
+    Lemma omap_concat_unnest2 d a a1 l :
+      omap_concat
+        (drec (("PDATA", d) :: ("a1", dcoll a1) :: nil))
+        (drec (("PBIND", a) :: nil)
+              :: map (fun x : data => drec (("PBIND", x) :: nil)) l)
+      =
+      Some (drec (("PBIND", a) :: ("PDATA", d) :: ("a1", dcoll a1) :: nil) ::
+                 (map (fun x : data => drec (("PBIND", x) :: ("PDATA", d) :: ("a1", dcoll a1) :: nil)) l)).
+    Proof.
+      unfold omap_concat; simpl.
+      rewrite lift_map_map_rec3; simpl; reflexivity.
+    Qed.
 
-  Lemma omap_concat_unnest2 d a a1 l :
-    omap_concat
-      (drec (("PDATA", d) :: ("a1", dcoll a1) :: nil))
-      (drec (("PBIND", a) :: nil)
-            :: map (fun x : data => drec (("PBIND", x) :: nil)) l)
-    =
-    Some (drec (("PBIND", a) :: ("PDATA", d) :: ("a1", dcoll a1) :: nil) ::
-               (map (fun x : data => drec (("PBIND", x) :: ("PDATA", d) :: ("a1", dcoll a1) :: nil)) l)).
-  Proof.
-    unfold omap_concat; simpl.
-    rewrite lift_map_map_rec3; simpl; reflexivity.
-  Qed.
-
-  Lemma lift_map_remove1 env l l2:
-    lift_map
-      (fun x : data =>
-         match x with
+    Lemma lift_map_remove1 env l l2:
+      lift_map
+        (fun x : data =>
+           match x with
            | drec r => Some (drec (rremove r "a1"))
            | _ => None
-         end)
-      (map
-         (fun x : data =>
-            drec
-              (("PBIND", env) :: ("PDATA", x) :: ("a1", dcoll l2) :: nil))
-         l)
-    =
-    Some (map (fun x: data => drec (("PBIND", env) :: ("PDATA", x) :: nil)) l).
-  Proof.
-    induction l; try reflexivity; simpl.
-    rewrite IHl; reflexivity.
-  Qed.
-  
+           end)
+        (map
+           (fun x : data =>
+              drec
+                (("PBIND", env) :: ("PDATA", x) :: ("a1", dcoll l2) :: nil))
+           l)
+      =
+      Some (map (fun x: data => drec (("PBIND", env) :: ("PDATA", x) :: nil)) l).
+    Proof.
+      induction l; try reflexivity; simpl.
+      rewrite IHl; reflexivity.
+    Qed.
+    
   Lemma lift_map_remove2 d l l2:
     lift_map
       (fun x : data =>
@@ -493,6 +1154,8 @@ Section cNRAEnv.
     (nraenv_core_eval ae env x) = (h ⊢ (nra_of_nraenv_core ae) @ₐ (nra_context_data env x) ⊣ constant_env).
   Proof.
     revert env x; nraenv_core_cases (induction ae) Case; simpl; intros.
+    - Case "cNRAEnvGetConstant"%string.
+      reflexivity.
     - Case "cNRAEnvID"%string.
       simpl; reflexivity.
     - Case "cNRAEnvConst"%string.
@@ -720,8 +1383,6 @@ Section cNRAEnv.
       rewrite IHae2. generalize ((h ⊢ (nra_of_nraenv_core ae2) @ₐ (nra_context_data env x) ⊣ constant_env)); intros.
       destruct o; try reflexivity; simpl.
       rewrite IHae1; reflexivity.
-    - Case "cNRAEnvGetConstant"%string.
-      reflexivity.
     - Case "cNRAEnvEnv"%string.
       reflexivity.
     - Case "cNRAEnvAppEnv"%string.
@@ -749,6 +1410,7 @@ Section cNRAEnv.
          (map (fun x0 : data => drec (("PBIND", x0) :: ("PDATA", x) :: nil))
               l)); try reflexivity; try congruence; simpl; destruct (lift_map (fun env' => (nraenv_core_eval ae env' x)) l); try reflexivity; try congruence.
   Qed.
+  End Semantics.
   
 End cNRAEnv.
 
@@ -768,6 +1430,9 @@ Section RcNRAEnv2.
     revert x c env.
     induction p; simpl; unfold olift, olift2; intros; trivial;
     try rewrite IHp; try rewrite IHp1; try rewrite IHp2; trivial.
+    - unfold edot. 
+      rewrite (assoc_lookupr_drec_sort (odt:=ODT_string)).
+      trivial.
     - match_destr.
       apply lift_oncoll_ext; intros.
       f_equal.
@@ -785,9 +1450,6 @@ Section RcNRAEnv2.
       rewrite IHp1; match_destr.
     - match_destr.
     - match_destr.
-    - unfold edot. 
-      rewrite (assoc_lookupr_drec_sort (odt:=ODT_string)).
-      trivial.
     - match_destr.
     - apply lift_oncoll_ext; intros.
       f_equal.
@@ -826,6 +1488,7 @@ Section RcNRAEnv2.
   Section FreeVars.
     Fixpoint nraenv_core_free_vars (q:nraenv_core) : list string :=
       match q with
+      | cNRAEnvGetConstant s => s :: nil
       | cNRAEnvID => nil
       | cNRAEnvConst rd => nil
       | cNRAEnvBinop _ q1 q2 =>
@@ -848,7 +1511,6 @@ Section RcNRAEnv2.
         nraenv_core_free_vars q1 ++ nraenv_core_free_vars q2
       | cNRAEnvApp q2 q1 =>
         nraenv_core_free_vars q1 ++ nraenv_core_free_vars q2
-      | cNRAEnvGetConstant s => s :: nil
       | cNRAEnvEnv => nil
       | cNRAEnvAppEnv q2 q1 =>
         nraenv_core_free_vars q1 ++ nraenv_core_free_vars q2
@@ -911,7 +1573,8 @@ Hint Resolve nraenv_core_eval_normalized.
 
 Tactic Notation "nraenv_core_cases" tactic(first) ident(c) :=
   first;
-  [ Case_aux c "cNRAEnvID"%string
+  [ Case_aux c "cNRAEnvGetConstant"%string
+  | Case_aux c "cNRAEnvID"%string
   | Case_aux c "cNRAEnvConst"%string
   | Case_aux c "cNRAEnvBinop"%string
   | Case_aux c "cNRAEnvUnop"%string
@@ -923,7 +1586,6 @@ Tactic Notation "nraenv_core_cases" tactic(first) ident(c) :=
   | Case_aux c "cNRAEnvEither"%string
   | Case_aux c "cNRAEnvEitherConcat"%string
   | Case_aux c "cNRAEnvApp"%string
-  | Case_aux c "cNRAEnvGetConstant"%string
   | Case_aux c "cNRAEnvEnv"%string
   | Case_aux c "cNRAEnvAppEnv"%string
   | Case_aux c "cNRAEnvMapEnv"%string].
